\documentclass[12pt]{article}
\usepackage{physics}

\begin{document}

\begin{center}
  \Large\textbf{Equations of Motion} \\
  \large\text{10/7/2025}
\end{center}

The original form of the equations from the mathematica notebook are given along with the simplifactions based on $V=0$, $h=0$, $h^{ij}=0$, and $f^{ij}=0$.

\section*{Eq.1}

\begin{align*}
& -2r^2 \sin\theta \left( h' - 2n_f \,(f^{11} + \phi)\, \vartheta_0' \right)
+\tfrac{1}{4} e^{\frac{1}{2}\nu - \lambda}
\\ &\Big(
 e^{\lambda} \big(
   r \big(
     r \sin\theta \\ &\big(
       -4h^2 
       + 2(f^{11} + \phi)(f^{22} + f^{33} + 2\phi) \\
       &- 2(f^{12})^2 - 2(f^{13})^2 
       + (h^{12})^2 + (h^{13})^2 + (h^{23})^2
     \big)
     - 2 f^{13} \cos\theta
   \big) \\
   &- 4\sin\theta
 \big)
 + 4\sin\theta \left(1 + r \nu_{r}\right)
\Big) \nonumber \\
&= \tfrac{1}{2} r^2 \sin\theta\, e^{-\frac{1}{2}\lambda - \nu}
  \sqrt{e^{\lambda + \nu}}
  \left( 2V(\vartheta_0)e^{\nu} + (\vartheta_0')^2 \right)
\end{align*}

Simplified:
\begin{align*}
& -4r^2 \sin\theta \left(n_f\phi\vartheta_0' \right)
+\tfrac{e^{\frac{\nu}{2} - \lambda}}{4}
\Big(
 e^{\lambda} \big(
   r \big(
     r \sin\theta \big(
       4\phi^2\big)
   \big)
   - 4\sin\theta
 \big)
 + 4\sin\theta \left(1 + r \nu_{r}\right)
\Big) \\
&= \tfrac{1}{2} r^2 \sin\theta\, e^{-\frac{\lambda}{2} - \nu}
  \sqrt{e^{\lambda + \nu}} (\vartheta_0')^2
\end{align*}

Finally:
\begin{align*}
-8r^2 \left(n_f\phi\vartheta_0' \right)
+2e^{\frac{\nu}{2} - \lambda}
\Big( e^{\lambda} \big(r^2\phi^2 - 1 \big) + r\nu_{r} + 1\Big)
= r^2 \, e^{-\frac{\nu}{2}}(\vartheta_0')^2
\end{align*}

\section*{Eq.2}

\begin{align*}
\frac{r}{2}\Big[
 & e^{\frac{\nu}{2}} \big(
   r \sin\theta \big(
     -2h\,h^{12}
     + f^{12}(f^{33} + \phi)
     - f^{13} f^{23}
   \big)
   - 2 f^{23} \cos\theta
 \big) \\
 &- f^{13} \sin\theta\, e^{\frac{\nu - \lambda}{2}}
 - r \sin\theta \big(
     (h^{12})' - 8n_f f^{12} \vartheta_0'
   \big)
\Big] = 0
\end{align*}

Simplified:
\begin{align*}
0 = 0
\end{align*}

\section*{Eq.3}

\begin{align*}
\frac{r}{2}\Big[
 & e^{\frac{\nu}{2}} \big(
   r \sin\theta \big(
     -2h\,h^{13}
     - f^{12} f^{23}
     + f^{13}(f^{22} + \phi)
   \big)
   + \cos\theta (f^{22} - f^{33})
 \big) \\
 &+ f^{12} \sin\theta\, e^{\frac{\nu - \lambda}{2}}
 - r \sin\theta \big(
     (h^{13})' - 8n_f f^{13} \vartheta_0'
   \big)
\Big] = 0
\end{align*}

Simplified:
\begin{align*}
  0 = 0
\end{align*}

\section*{Eq.4}

\begin{align*}
\frac{1}{4} r \Big[
 & e^{\frac{1}{2}\nu} \big(
   2h^{12}\cos\theta
   - r\sin\theta \big[
       h^{23}\big(2f^{11} + f^{22} + f^{33} + 4\phi\big)
       - f^{12}h^{13}
       + f^{13}h^{12}
     \big]
 \big) \\
 &- 8n_f r\, h^{23} \sin\theta\, \vartheta_0'
 + 4 e^{-\frac{1}{2}\lambda} \sin\theta\, e^{\frac{1}{2}\nu}\, r h
   (\nu_r + \lambda_\tau)
\Big] = 0
\end{align*}

Simplified:
\begin{align*}
  0 = 0
\end{align*}

\section*{Eq.5}

\begin{align*}
\frac{1}{4} \sin\theta \Big[
 & e^{\frac{\nu}{2}} f^{13} \left( 4 + r \nu_r \right)
 + 2 e^{\frac{\lambda}{2}} r \\ &\Big(
     e^{\frac{\nu}{2}} \big(
       2h\,h^{12}
       + f^{12}(f^{33} + \phi)
       - f^{13} f^{23}
     \big)
     + (h^{12})'
     + 8n_f f^{12} \vartheta_0'
     + h^{12} \lambda_\tau
   \Big)
\Big] \\ &= 0
\end{align*}

Simplified:
\begin{align*}
0 = 0
\end{align*}

\section*{Eq.6}

\begin{align*}
\frac{1}{4} e^{-\frac{\lambda + \nu}{2}} \Big[
 & e^{\frac{\lambda + \nu}{2}} \sin\theta\, f^{23}\left(2 + r\nu_r\right)
 - e^{\nu} \sin\theta
   \left( \lambda_r - \nu_r \right) \left(2 + r\nu_r\right)
 - 2r (\nu_r)_r\\
 & + e^{\lambda} e^{\nu} \\
   &\Big(
     r \sin\theta
       \big[
         -4h^2
         + 2(f^{22} + \phi)(f^{11} + f^{33} + 2\phi) \\
         &- 2(f^{12})^2 - 2(f^{23})^2
         + (h^{12})^2 + (h^{13})^2 + (h^{23})^2
       \big]
     + 2f^{13}\cos\theta
   \Big) \\
 & - 4 e^{\frac{\nu}{2}} r \sin\theta
   \Big(
     2h'
     - 4n_f (f^{22} + \phi)\vartheta_0'
     + h\lambda_\tau
   \Big) \\
 &- r \sin\theta
   \Big[
     (\lambda_\tau)_\tau
     - \lambda_\tau \nu_\tau
     + 2(\lambda_\tau)_\tau
   \Big]
\Big]
\nonumber \\
&= \frac{1}{2} r \sin\theta\, e^{-\nu} \sqrt{e^{\lambda + \nu}}
   \left(2V(\vartheta_0)e^{\nu} + (\vartheta_0')^2\right)
\end{align*}

Simplified:

\begin{align*}
\frac{1}{4} e^{-\frac{\lambda + \nu}{2}} \Big[
 &- e^{\nu} \sin\theta
   \left( \lambda_r - \nu_r \right) \left(2 + r\nu_r\right) \\
 & - 2r (\nu_r)_r\\
 & + 4 e^{\lambda} e^{\nu} r\phi^2 \sin\theta \\
 & + 16 e^{\frac{\nu}{2}} r n_f\phi\vartheta_0' \sin\theta\\
 & - r \sin\theta
   \Big[
     (\lambda_\tau)_\tau
     - \lambda_\tau \nu_\tau
     + 2(\lambda_\tau)_\tau
   \Big]
\Big] \\
&= \frac{1}{2} r \sin\theta\, e^{-\nu} \sqrt{e^{\lambda + \nu}}
   \left((\vartheta_0')^2\right)
\end{align*}

Finally:
\begin{align*}
e^{-\frac{\lambda + \nu}{2}} \Big[
 &- \frac{e^{\nu}}{2} \left( \lambda_r - \nu_r \right) \left(\frac{2}{r} + \nu_r\right)
 - \frac{(\nu_r)_r}{\sin\theta} \\
 &+ 2 e^{\lambda} e^{\nu} \phi^2
 + 8 e^{\frac{\nu}{2}} n_f\phi\vartheta_0'
 - \frac{(\lambda_\tau)_\tau}{2} + \frac{\lambda_\tau \nu_\tau}{2} -(\lambda_\tau)_\tau
\Big] = e^\frac{\lambda - \nu}{2} (\vartheta_0')^2
\end{align*}

\section*{Eq.7}

\begin{align*}
\frac{1}{4} \Big[
 & - e^{\frac{\nu}{2}} \sin\theta
   \Big(
     2(f^{11} - f^{33})
     + r(f^{11} + f^{22} + 2\phi)\nu_r
   \Big) \\
 & + e^{\frac{\lambda}{2}}
   \Big(
     -2 e^{\frac{\nu}{2}} \big[
       r \sin\theta \big(
         2h\,h^{23}
         - f^{23}(f^{11} + \phi)
         + f^{12}f^{13}
       \big)
       + f^{12}\cos\theta
     \big] \\
 & \quad - r \sin\theta
       \big[
         2(h^{23})'
         - 16n_f f^{23}\vartheta_0'
         + h^{23}\lambda_\tau
       \big]
   \Big)
\Big] = 0
\end{align*}

Simplified:
\begin{align*}
\frac{1}{4} \Big[- e^{\frac{\nu}{2}} \sin\theta (2r\phi\nu_r) \Big] &= 0
\end{align*}

Finally:
\begin{align*}
- \frac{r \phi \nu_r}{2} e^{\frac{\nu}{2}} \sin\theta &= 0
\end{align*}

\section*{Eq.8}

\begin{align*}
\frac{1}{4} \sin\theta \Big[
 & -2 e^{\frac{\nu}{2}}
   h^{12}\left(1 + r\nu_r\right) \\
 & + e^{\frac{\lambda}{2}} r
   \Big(
     e^{\frac{\nu}{2}} \big[
       h^{13}(f^{11} + 2f^{22} + f^{33} + 4\phi)
       - f^{12}h^{23}
       - f^{23}h^{12}
     \big] \\
     & \quad + 8n_f\,h^{13}\,\vartheta_0'
     - f^{13}\lambda_\tau
   \Big)
\Big] = 0
\end{align*}

Simplified:
\begin{align*}
  0 = 0
\end{align*}

\section*{Eq.9}

\begin{align*}
\frac{1}{4} \Big[
 & - e^{\frac{\nu}{2}} f^{12} \left( 4 + r\nu_r \right) \\
 & + 2 e^{\frac{\lambda}{2}} r
   \Big(
     e^{\frac{\nu}{2}} \big(
       2h\,h^{13} - f^{12} f^{23} + f^{13}(f^{22} + \phi)
     \big) \\
     & \quad + (h^{13})'
     + 8 n_f f^{13} \vartheta_0'
     + h^{13} \lambda_\tau
   \Big)
\Big] = 0
\end{align*}

Simplified:
\begin{align*}
  0 = 0
\end{align*}

\section*{Eq.10}

\begin{align*}
\frac{1}{4} \Big[
 & e^{\frac{\nu}{2}} \Big(
     2(f^{11} - f^{22}) + r(f^{11} + f^{33} + 2\phi)\nu_r
   \Big) \\
 & + e^{\frac{\lambda}{2}} r \Big(
     -2 e^{\frac{\nu}{2}} \Big(
       -2 h\, h^{23} - f^{23}(f^{11} + \phi) + f^{12} f^{13}
     \Big) \\
     & \quad + 2 (h^{23})'
     + 16 n_f f^{23} \vartheta_0'
     + h^{23} \lambda_\tau
   \Big)
\Big] = 0
\end{align*}

Simplified:
\begin{align*}
\frac{1}{4} \Big[
 & e^{\frac{\nu}{2}} \Big(
     r(2\phi)\nu_r
   \Big)
\Big] = 0
\end{align*}

Finally:
\begin{align*}
\frac{r\phi\nu_r}{2} e^{\frac{\nu}{2}} = 0
\end{align*}

\section*{Eq.11}

\begin{align*}
\frac{1}{4} e^{-\frac{\lambda + \nu}{2}} \Big[
 & e^{\nu} r \Big(
     - e^{\lambda} \\ & \quad \Big(
       4h^2 - 2(f^{33} + \phi)(f^{11} + f^{22} + 2\phi) \\
       & + 2(f^{13})^2 + 2(f^{23})^2
       - (h^{12})^2 - (h^{13})^2 - (h^{23})^2
     \Big) \\
 & \quad - 2 \lambda_r + 2 \nu_r
       - e^{\frac{\lambda}{2}} f^{23}\left(2 + r\nu_r\right) \\
 & \quad + r \Big(
       - \lambda_r \nu_r
       + (\nu_r)^2
       + 2 (\nu_r)_r
     \Big)
   \Big) \\
 & - 4 e^{\lambda + \frac{\nu}{2}} r
   \Big(
     2 h' - 4 n_f (f^{33} + \phi) \vartheta_0' + h\lambda_\tau
   \Big) \\
 & - e^{\lambda} r
   \Big[
     \left(\lambda_\tau\right)^2
     - \lambda_\tau \nu_\tau
     + 2 (\lambda_\tau)_\tau
   \Big]
\Big] \\
&= \frac{1}{2} r e^{-\nu} \sqrt{e^{\lambda + \nu}}
   \left( 2 V(\vartheta_0) e^{\nu} + (\vartheta_0')^2 \right)
\end{align*}

Simplified:
\begin{align*}
\frac{1}{4} e^{-\frac{\lambda + \nu}{2}} \Big[
 & e^{\nu} \Big(
     - 4e^{\lambda}\phi^2 - 2 \lambda_r + 2 \nu_r 
      + r ( - \lambda_r \nu_r + (\nu_r)^2 + 2 (\nu_r)_r )
   \Big) \\
 & + 16 n_f \phi e^{\lambda + \frac{\nu}{2}} \vartheta_0' \\
& - e^{\lambda}
   (
     \left(\lambda_\tau\right)^2
     - \lambda_\tau \nu_\tau
     + 2 (\lambda_\tau)_\tau
   )
\Big] \\
&= \frac{1}{2} e^\frac{\lambda - \nu}{2}(\vartheta_0')^2
\end{align*}

Finally:
\begin{align*}
e^{-\frac{\lambda + \nu}{2}} \Big[
 & e^{\nu} \Big(
     - 2e^{\lambda}\phi^2 - \lambda_r + \nu_r 
      + \frac{r}{2} ( - \lambda_r \nu_r + (\nu_r)^2 + 2 (\nu_r)_r )
   \Big) \\
 & + 8 n_f \phi e^{\lambda + \frac{\nu}{2}} \vartheta_0' - \frac{e^{\lambda}}{2} (\left(\lambda_\tau\right)^2 - \lambda_\tau \nu_\tau + 2 (\lambda_\tau)_\tau)
\Big] = e^\frac{\lambda - \nu}{2}(\vartheta_0')^2
\end{align*}

\section*{Eq.12}

\begin{align*}
\frac{1}{4} \Big[
 & -2 e^{\frac{\nu}{2}} \, h^{13} \left( 1 + r \nu_r \right) \\
 & + e^{\frac{\lambda}{2}} r \Big(
   - e^{\frac{\nu}{2}} \big[
       h^{12}(f^{11} + f^{22} + 2f^{33} + 4\phi)
       + f^{13} h^{23}
       - f^{23} h^{13}
     \big] \\
   & \quad - 8 n_f \, h^{12} \vartheta_0'
   + f^{12}\lambda_\tau
 \Big)
\Big] = 0
\end{align*}

Simplified:
\begin{align*}
  0 = 0
\end{align*}

\section*{Eq.13}

\begin{align*}
\frac{1}{2} e^{-\frac{\nu}{2}} \Big[
  & r e^{\frac{\lambda + \nu}{2}} 
  \Big(
    r \sin\theta \big(
      -f^{12}h^{13}
      + f^{13}h^{12}
      - h^{23}(f^{22} + f^{33} + 2\phi)
    \big)
    - h^{12}\cos\theta
  \Big) \\
  & - 2r \sin\theta \lambda_\tau
\Big] = 0
\end{align*}

Simplify:
\begin{align*}
\frac{1}{2} e^{-\frac{\nu}{2}} \Big[ - 2r \sin\theta \lambda_\tau \Big] = 0
\end{align*}

Finally:
\begin{align*}
- r \lambda_\tau e^{-\frac{\nu}{2}}\sin\theta = 0
\end{align*}

\section*{Eq.14}

\begin{align*}
\frac{1}{2} r \sin\theta \Big[
  r e^{\frac{\lambda}{2}}
  \big(
    h^{13}(f^{11} + f^{33} + 2\phi)
    + f^{12}h^{23}
    + f^{23}h^{12}
  \big)
  + h^{12}
\Big] = 0
\end{align*}

Simplify:
\begin{align*}
  0 = 0
\end{align*}

\section*{Eq.15}

\begin{align*}
\frac{1}{2} r \sin\theta \Big[
  h^{13}
  - r e^{\frac{\lambda}{2}}
  \big(
    h^{12}(f^{11} + f^{22} + 2\phi)
    - f^{13}h^{23}
    + f^{23}h^{13}
  \big)
\Big] = 0
\end{align*}

Simplify:
\begin{align*}
  0 = 0
\end{align*}

\section*{Eq.16}

\begin{align*}
\frac{1}{4} e^{-\frac{\lambda + \nu}{2}} \sin\theta 
\Big[
  &e^{\frac{\nu}{2}}
  \Big(
    4 \\
    &- e^{\lambda}\Big(
      r^2 \big(
        12 h^2
        - 8\phi(f^{11} + f^{22} + f^{33})
        - 4 f^{33}(f^{11} + f^{22}) \\
        & \quad - 4 f^{11} f^{22}
        + 4 (f^{12})^2 + 4 (f^{13})^2 + 4 (f^{23})^2 \\
        & \quad + (h^{12})^2 + (h^{13})^2 + (h^{23})^2
        - 12\phi^2
      \big)
      + 4
    \Big)
    - 4r\lambda_r
  \Big) \\
  & - 4 e^{\lambda} r^2 h\,\lambda_\tau
\Big] \\
& =
\frac{1}{2} r^2 \sin\theta\,
e^{-\tfrac{3}{2}\nu}
\sqrt{e^{\lambda + \nu}}
\Big(
  2V(\vartheta_0)e^{\nu}
  - (\vartheta_0')^2
\Big)
\end{align*}

Simplify:
\begin{align*}
\frac{1}{4} e^{-\frac{\lambda + \nu}{2}} \sin\theta 
\Big[
  &e^{\frac{\nu}{2}}
  \Big(
    4 - e^{\lambda}\Big(
      r^2 \big(- 12\phi^2\big) + 4
    \Big) - 4r\lambda_r
  \Big) \Big] \\
& =
\frac{1}{2} r^2 \sin\theta\,
e^{-\tfrac{3}{2}\nu}
\sqrt{e^{\lambda + \nu}}
\Big(
  - (\vartheta_0')^2
\Big)
\end{align*}

Finally:
\begin{align*}
2 
\Big(
  e^{\lambda}(3r^2\phi^2 - 1) - r\lambda_r + 1
\Big)
= - r^2 
e^{\lambda-\nu} (\vartheta_0')^2
\end{align*}

\section*{List of Equations}

\begin{align*}
-8r^2 \left(n_f\phi\vartheta_0' \right)
+2e^{\frac{\nu}{2} - \lambda}
\Big( e^{\lambda} \big(r^2\phi^2 - 1 \big) + r\nu_{r} + 1\Big)
= r^2 \, e^{-\frac{\nu}{2}}(\vartheta_0')^2
\end{align*}

\begin{align*}
e^{-\frac{\lambda + \nu}{2}} \Big[
 &- \frac{e^{\nu}}{2} \left( \lambda_r - \nu_r \right) \left(\frac{2}{r} + \nu_r\right)
 - \frac{(\nu_r)_r}{\sin\theta} \\
 &+ 2 e^{\lambda} e^{\nu} \phi^2
 + 8 e^{\frac{\nu}{2}} n_f\phi\vartheta_0'
 - \frac{(\lambda_\tau)_\tau}{2} + \frac{\lambda_\tau \nu_\tau}{2} -(\lambda_\tau)_\tau
\Big] = e^\frac{\lambda - \nu}{2} (\vartheta_0')^2
\end{align*}

\begin{align*}
- \frac{r \phi \nu_r}{2} e^{\frac{\nu}{2}} \sin\theta &= 0
\end{align*}

\begin{align*}
\frac{r\phi\nu_r}{2} e^{\frac{\nu}{2}} = 0
\end{align*}

\begin{align*}
e^{-\frac{\lambda + \nu}{2}} \Big[
 & e^{\nu} \Big(
     - 2e^{\lambda}\phi^2 - \lambda_r + \nu_r 
      + \frac{r}{2} ( - \lambda_r \nu_r + (\nu_r)^2 + 2 (\nu_r)_r )
   \Big) \\
 & + 8 n_f \phi e^{\lambda + \frac{\nu}{2}} \vartheta_0' - \frac{e^{\lambda}}{2} (\left(\lambda_\tau\right)^2 - \lambda_\tau \nu_\tau + 2 (\lambda_\tau)_\tau)
\Big] = e^\frac{\lambda - \nu}{2}(\vartheta_0')^2
\end{align*}

\begin{align*}
- r \lambda_\tau e^{-\frac{\nu}{2}}\sin\theta = 0
\end{align*}

\begin{align*}
2 
\Big(
  e^{\lambda}(3r^2\phi^2 - 1) - r\lambda_r + 1
\Big)
= - r^2 
e^{\lambda-\nu} (\vartheta_0')^2
\end{align*}

\end{document}