\documentclass[12pt]{article}
\usepackage{physics}

\begin{document}
\begin{center}
  \Large\textbf{Friedman Equations of Motion after substitution} \\
  \large\text{10/13/2025}
\end{center}

After substituting the known form of $\phi$ from the pre-substitution TEOM notes as well as the other constraints, the Friedman EOMs have been recalculated. $V(\vartheta_0)=0$ is enforced now. The equations are presented:

\section*{Equation 1}

\begin{align*}
\sin\theta &\Big(
  4 n f r^2 \, \vartheta_0' 
  \, n f \, \vartheta_0' (- e^{-\nu/2}) \\
  & \qquad + e^{\nu/2 - \lambda} \Big(
      1 + r \, \nu_r + e^{\lambda} \big( r^2 ((n f \, \vartheta_0' (- e^{-\nu/2}))^2 - 0^2) - 1 \big)
    \Big)
\Big) \\
& = \frac{1}{2} r^2 \sin\theta \, e^{-\lambda/2 - \nu} \sqrt{e^{\lambda+\nu}} \Big( 2 V(\vartheta_0) e^{\nu} + (\vartheta_0')^2 \Big)  \\  \\
&4 n^2 f^2 r^2
  \, (\vartheta_0')^2 (- e^{-\nu/2})  \\
  & \qquad + e^{\nu/2 - \lambda} \Big(
      1 + r \, \nu_r + e^{\lambda} \big( r^2 ((n f \, \vartheta_0' (- e^{-\nu/2}))^2) - 1 \big)
    \Big) \\
& = \frac{1}{2} r^2 e^{-\nu/2} (\vartheta_0')^2  \\  \\
&-8 n^2 f^2 r^2
  \, (\vartheta_0')^2 \\
  & \qquad + 2e^{\nu - \lambda} \Big(
      1 + r \, \nu_r + e^{\lambda} \big( r^2 ((n f \, \vartheta_0' (- e^{-\nu/2}))^2) - 1 \big)
    \Big) \\
& = r^2 (\vartheta_0')^2 
\end{align*}

Focusing specifically on this term:
\begin{align*}
  &2e^{\nu - \lambda} \Big(
      1 + r \, \nu_r + e^{\lambda} \big( r^2 ((n f \, \vartheta_0' (- e^{-\nu/2}))^2) - 1 \big)
    \Big) \\
  &2e^{\nu - \lambda} + 2e^{\nu - \lambda}r \nu_r + 2e^{\nu} \big( r^2 n^2 f^2 \, (\vartheta_0')^2 (e^{-\nu}) - 1 \big) \\
  &2e^{\nu - \lambda} + 2e^{\nu - \lambda}r \nu_r + 2 r^2 n^2 f^2 \, (\vartheta_0')^2 - 2e^{\nu}
\end{align*}

Substituting back into the equation:

\begin{align}
  -8 n^2 f^2 r^2 (\vartheta_0')^2 + 2e^{\nu - \lambda} + 2e^{\nu - \lambda}r \nu_r &+ 2 r^2 n^2 f^2 \, (\vartheta_0')^2 - 2e^{\nu} = r^2 (\vartheta_0')^2 \nonumber \\ \nonumber \\
  -6 n^2 f^2 r^2 (\vartheta_0')^2 + 2e^{\nu - \lambda} &+ 2e^{\nu - \lambda}r \nu_r - 2e^{\nu} = r^2 (\vartheta_0')^2 \nonumber \\ \nonumber \\
  2e^{\nu - \lambda} + 2e^{\nu - \lambda}r \nu_r - 2e^{\nu} &= r^2 (\vartheta_0')^2 + 6 n^2 f^2 r^2 (\vartheta_0')^2 \nonumber \\ \nonumber \\
  2e^{\nu} \left(e^{-\lambda} + e^{-\lambda}r \nu_r - 1\right) &= r^2  \left(1 + 6 n^2 f^2\right)(\vartheta_0')^2
\end{align}

\section*{Equation 2}

\begin{align}
  e^{-\lambda/2} r \sin\theta \left(e^{\nu/2}r(0)(\nu_r) + \lambda_\tau \right) &= 0 \nonumber \\
  e^{-\lambda/2} r \sin\theta (\lambda_\tau) &= 0 \nonumber \\
  \lambda_\tau &= 0
\end{align}

This constraint will be applied to the rest of the equations.

\section*{Equation 3}

\begin{align}
&\frac{1}{4} e^{\frac{-\lambda-\nu}{2}} \sin\theta \Big[
 - e^{\lambda} r \big( \lambda_\tau^2 - \lambda_\tau \nu_\tau + 2 \lambda_{\tau\tau} \big) - 4 e^{\lambda+\frac{\nu}{2}} r \big( 0\lambda_\tau - 4 n f \vartheta_0'n f \vartheta_0' (-e^{-\frac{1}{2}\nu}) \big) \nonumber\\
 & \quad + e^{\nu} \big( -4 (0)^2 r e^{\lambda} + 2 \nu_r - \lambda_r (2 + r \nu_r) \nonumber\\
 & \qquad\qquad + r \big( \nu_r^2 + 2 \nu_{rr} + 4 e^{\lambda} (n f \vartheta_0' (-e^{-\frac{1}{2}\nu}))^2 \big) \big)
\Big] \nonumber \\
& = \frac{1}{2} r \sin\theta e^{-\nu} \sqrt{e^{\lambda+\nu}} \left( 2V e^{\nu} + (\vartheta_0')^2 \right) \nonumber \\ \nonumber \\
&\frac{1}{2} e^{\frac{1}{2}(-\lambda-\nu)} \Big[
 - 4 e^{\lambda+\frac{1}{2}\nu} r \big(4 n^2 f^2 (\vartheta_0')^2 e^{-\frac{1}{2}\nu} \big) \nonumber \\
& \quad + e^{\nu} \big(2 \nu_r - \lambda_r (2 + r \nu_r) + r \big( \nu_r^2 + 2 \nu_{rr} + 4 e^{\lambda} (n^2 f^2 (\vartheta_0')^2 e^{-\nu}) \big) \big)
\Big] \nonumber \\
& = r e^{-\frac{\nu}{2} + \frac{\lambda}{2}} (\vartheta_0')^2 \nonumber \\ \nonumber \\
& - 4 e^{\frac{1}{2}\nu} r \big(4 n^2 f^2 (\vartheta_0')^2 e^{-\frac{1}{2}\nu} \big) \nonumber \\
& \quad + e^{\nu-\lambda} \big(2 \nu_r - \lambda_r (2 + r \nu_r) + r \big( \nu_r^2 + 2 \nu_{rr} + 4 e^{\lambda} (n^2 f^2 (\vartheta_0')^2 e^{-\nu}) \big) \big) \nonumber \\
& = 2r (\vartheta_0')^2 \nonumber \\ \nonumber \\
&e^{\nu-\lambda} \big(2 \nu_r - \lambda_r (2 + r \nu_r) + r \big( \nu_r^2 + 2 \nu_{rr} + 4 e^{\lambda} (n^2 f^2 (\vartheta_0')^2 e^{-\nu}) \big) \big) \nonumber \\
& = 2r (\vartheta_0')^2 + 16 r n^2 f^2 (\vartheta_0')^2 \nonumber \\ \nonumber \\
&e^{\nu-\lambda} \big(2 \nu_r - \lambda_r (2 + r \nu_r) + r\nu_r^2 + 2r \nu_{rr} + 4r e^{\lambda-\nu} n^2 f^2 (\vartheta_0')^2 \big) \nonumber \\
& = 2r (\vartheta_0')^2 + 16 r n^2 f^2 (\vartheta_0')^2 \nonumber \\ \nonumber \\
&\frac{1}{2}e^{\nu-\lambda} \big(2 \nu_r - \lambda_r (2 + r \nu_r) + r\nu_r^2 + 2r \nu_{rr} \big) = r (\vartheta_0')^2 + 6 r n^2 f^2 (\vartheta_0')^2 \nonumber \\ \nonumber \\
&e^{\nu-\lambda} \big(\nu_r - \frac{1}{2} \lambda_r (2 + r \nu_r) + \frac{1}{2}r\nu_r^2 + r\nu_{rr} \big) = r \left(1 + 6 n^2 f^2\right) (\vartheta_0')^2
\end{align}


\section*{Equation 4}

\begin{align}
-\frac{1}{2} e^{\frac{1}{2} \nu} r \sin(\theta) 
\left(
    \nu_r \left( 
        - e^{-\frac{1}{2} \nu} \vartheta_0' nf
    \right)
    + 2 \left(
        \frac{1}{2} e^{-\frac{1}{2} \nu} nf \vartheta_0' \nu_r
    \right)
\right) &= 0 \nonumber \\ 
    - \nu_r e^{-\frac{1}{2} \nu} \vartheta_0' nf
    + e^{-\frac{1}{2} \nu} nf \vartheta_0' \nu_r &= 0 \nonumber \\
0 &= 0
\end{align}

\section*{Equation 5}

Equation 5 is functionally the same structure as Equation 4 and yields:
\begin{align}
  0 = 0
\end{align}

\section*{Equation 6}

\begin{align*}
&\frac{1}{4} e^{\frac{1}{2}(-\lambda - \nu)} 
\Big[ 
     - e^{\lambda} r 
    \big(
        \lambda_\tau^2 
        - \lambda_\tau \nu_\tau
        + 2 \lambda_{\tau\tau}
    \big) \\
    & \quad - 4 e^{\lambda + \frac{1}{2}\nu} r 
    \big(
        0 \lambda_\tau 
        - 4 \, nf \, \vartheta_0' \, nf \, \vartheta_0' (- e^{-\frac{1}{2}\nu})
    \big) \\
    & \quad + e^{\nu} 
    \Big(
        -4 (0)^2 r e^{\lambda}
        + 2 \nu_r
        - \lambda_r
        \big(2 + r \nu_r \big) \\
        & \qquad + r \big(
            \nu_r^2 
            + 2 \nu_{rr} 
            + 4 e^{\lambda} 
            (nf \, \vartheta_0' (- e^{-\frac{1}{2}\nu}))^2
        \big)
    \Big)
\Big] \\
&= \frac{1}{2} r e^{-\nu} \sqrt{e^{\lambda + \nu}} 
\left(
    2 V(\vartheta_0) e^{\nu} + (\vartheta_0')^2
\right) \\ \\
&\frac{1}{2} e^{\frac{1}{2}(-\lambda - \nu)} 
\Big[  - 4 e^{\lambda + \frac{1}{2}\nu} r 
    \big(
        - 4 \, nf \, \vartheta_0' \, nf \, \vartheta_0' (- e^{-\frac{1}{2}\nu})
    \big) \\
    & \quad + e^{\nu} 
    \Big(
        2 \nu_r
        - \lambda_r
        \big(2 + r \nu_r \big)
        + r \big(
            \nu_r^2 
            + 2 \nu_{rr} 
            + 4 e^{\lambda} 
            (nf \, \vartheta_0' (- e^{-\frac{1}{2}\nu}))^2
        \big)
    \Big)
\Big] \\
&= r e^{-\nu} \sqrt{e^{\lambda + \nu}} (\vartheta_0')^2 \\ \\
&\frac{1}{2} e^{\frac{1}{2}(-\lambda - \nu)} 
\Big[  - 4 e^{\lambda + \frac{1}{2}\nu} r 
    \big(
        - 4 n^2 f^2 (\vartheta_0')^2 (- e^{-\frac{1}{2}\nu})
    \big) \\
    & \quad + e^{\nu} 
    \Big(
        2 \nu_r
        - \lambda_r
        \big(2 + r \nu_r \big)
        + r \big(
            \nu_r^2 
            + 2 \nu_{rr} 
            + 4 e^{\lambda-\nu} n^2 f^2 (\vartheta_0')^2
        \big)
    \Big)
\Big] \\
&= r e^{(\lambda-\nu)/2} (\vartheta_0')^2
\end{align*}

\begin{align*}
&\frac{1}{2}
\Big[- 4 e^{\frac{1}{2}\nu} r 
    \big(
        - 4 n^2 f^2 (\vartheta_0')^2 (- e^{-\frac{1}{2}\nu})
    \big) \\
    & \quad + e^{\nu-\lambda} 
    \Big(
        2 \nu_r
        - \lambda_r
        \big(2 + r \nu_r \big)
        + r \big(
            \nu_r^2 
            + 2 \nu_{rr} 
            + 4 e^{\lambda-\nu} n^2 f^2 (\vartheta_0')^2
        \big)
    \Big)
\Big] \\
&= r (\vartheta_0')^2 \\ \\
&\frac{1}{2}
\Big[-16  r n^2 f^2 (\vartheta_0')^2 \\
    & \quad +
        2 e^{\nu-\lambda} \nu_r
        - e^{\nu-\lambda} \lambda_r
        \big(2 + r \nu_r \big)
        + e^{\nu-\lambda} r\nu_r^2 
        + 2e^{\nu-\lambda} r \nu_{rr} 
        + 4 r n^2 f^2 (\vartheta_0')^2
\Big] \\
&= r (\vartheta_0')^2 \\ \\
&-6 r n^2 f^2 (\vartheta_0')^2 +
e^{\nu-\lambda} \nu_r
- \frac{1}{2} e^{\nu-\lambda} \lambda_r
\big(2 + r \nu_r \big)
+ \frac{1}{2} e^{\nu-\lambda} r\nu_r^2 
+ e^{\nu-\lambda} r \nu_{rr} \\
&= r (\vartheta_0')^2 \\ \\
& e^{\nu-\lambda} \left(\nu_r
- \frac{1}{2} \lambda_r
\big(2 + r \nu_r \big)
+ \frac{1}{2} r\nu_r^2 
+ r \nu_{rr} \right)
= r(1 + 6 n^2 f^2 ) (\vartheta_0')^2
\end{align*}

\begin{align}
e^{\nu-\lambda} \left(\nu_r - \lambda_r - \frac{1}{2} r \nu_r \left( \lambda_r + \nu_r \right) + r \nu_{rr} \right) = r(1 + 6 n^2 f^2 ) (\vartheta_0')^2
\end{align}

\section*{Equation 7}

Equation 7 is functionally the same structure as Equation 2 and yields:
\begin{align}
  \lambda_\tau = 0
\end{align}

\section*{Equation 8}

\begin{align}
&e^{\frac{1}{2}(-\lambda-\nu)}\sin\theta\Big[
 -e^{\lambda} r^2 0 \lambda_\tau \nonumber \\
 & \quad - e^{\frac{1}{2}\nu}\Big(
    -1 + r \lambda_r
    + e^{\lambda}\Big(3 r^2\big(0^2 - (n f \vartheta_0' (-e^{-\frac{1}{2}\nu}))^2\big) + 1\Big)
   \Big)
\Big] \nonumber\\
&= \frac{1}{2} r^2 \sin\theta\, e^{-\frac{3}{2}\nu} \sqrt{e^{\lambda+\nu}}\Big(2 V e^{\nu} - \vartheta_0'^2\Big) \nonumber \\ \nonumber \\
&2e^{\frac{1}{2}(-\lambda-\nu)} \Big[
 - e^{\frac{1}{2}\nu}\Big(
    -1 + r \lambda_r
    + e^{\lambda}\Big(-3 r^2(n f \vartheta_0' (-e^{-\frac{1}{2}\nu}))^2 + 1\Big)
   \Big)
\Big] \nonumber\\
&= -r^2 e^{-\nu + \frac{\lambda}{2}} (\vartheta_0')^2 \nonumber \\ \nonumber \\
&2e^{-\lambda + \nu}\Big(
    -1 + r \lambda_r
    + e^{\lambda}\Big(-3 r^2 n^2 f^2 (\vartheta_0')^2 e^{-\nu} + 1\Big)
   \Big) = r^2 (\vartheta_0')^2 \nonumber \\ \nonumber \\
&2e^{-\lambda + \nu}\Big(
  -1 + r \lambda_r -3 r^2 n^2 f^2 (\vartheta_0')^2 e^{\lambda-\nu} + e^{\lambda} \Big) = r^2 (\vartheta_0')^2 \nonumber \\ \nonumber \\
&2e^{-\lambda + \nu}\Big(
  -1 + r \lambda_r + e^{\lambda} \Big) = r^2 (\vartheta_0')^2 + 6 r^2 n^2 f^2 (\vartheta_0')^2 \nonumber \\ \nonumber \\
&2e^{\nu-\lambda}\Big(
  -1 + r \lambda_r + e^{\lambda} \Big) = r^2 (1 + 6 n^2 f^2) (\vartheta_0')^2
\end{align}

\section*{List of Equations}

\begin{align}
  2e^{\nu} \left(e^{-\lambda} + e^{-\lambda}r \nu_r - 1\right) &= r^2(1 + 6 n^2 f^2)(\vartheta_0')^2 \\ \nonumber \\
  \lambda_\tau &= 0 \\ \nonumber \\
  e^{\nu-\lambda} \big(\nu_r - \frac{1}{2} \lambda_r (2 + r \nu_r) + \frac{1}{2}r\nu_r^2 + r\nu_{rr} \big) &= r (1 + 6 n^2 f^2) (\vartheta_0')^2 \\ \nonumber \\
  e^{\nu-\lambda} \left(\nu_r - \lambda_r - \frac{1}{2} r \nu_r \left( \lambda_r + \nu_r \right) + r \nu_{rr} \right) &= r(1 + 6 n^2 f^2 ) (\vartheta_0')^2 \\ \nonumber \\
  2e^{\nu-\lambda}\Big(
  -1 + r \lambda_r + e^{\lambda} \Big) &= r^2 (1 + 6 n^2 f^2) (\vartheta_0')^2
\end{align}

Equations 9 and 13 can be equated to each other:

\begin{align*}
  2e^{\nu} \left(e^{-\lambda} + e^{-\lambda}r \nu_r - 1\right) &= 2e^{\nu-\lambda}\Big(
  -1 + r \lambda_r + e^{\lambda} \Big) \\
  e^{-\lambda} + e^{-\lambda}r \nu_r - 1 &= e^{-\lambda}\Big( -1 + r \lambda_r + e^{\lambda} \Big) \\
  e^{-\lambda} + e^{-\lambda}r \nu_r - 1 &= -e^{-\lambda} + e^{-\lambda} r \lambda_r \\
  2e^{-\lambda} + e^{-\lambda}r \nu_r - e^{-\lambda} r \lambda_r &= 1 \\
  e^{-\lambda} \left(2 + r\nu_r -  r\lambda_r\right) &= 1 \\
  2 + r \left(\nu_r - \lambda_r\right) &= e^{\lambda}
\end{align*}
\begin{align}
  \nu_r - \lambda_r &= \frac{e^{\lambda} - 2}{r}
\end{align}

Equations 11 and 12 can be equated to each other:

\begin{align*}
  e^{\nu-\lambda} \big(\nu_r - \frac{\lambda_r}{2} (2 + r \nu_r) + \frac{r}{2}\nu_r^2 + r\nu_{rr} \big) &= e^{\nu-\lambda} (\nu_r - \lambda_r - \frac{r}{2} \nu_r (\lambda_r + \nu_r ) + r\nu_{rr}) \\
  \nu_r - \frac{\lambda_r}{2} (2 + r \nu_r) + \frac{r}{2}\nu_r^2 + r\nu_{rr} &= \nu_r - \lambda_r - \frac{r}{2} \nu_r (\lambda_r + \nu_r ) + r\nu_{rr} \\
  - \frac{\lambda_r}{2} (2 + r \nu_r) + \frac{r}{2}\nu_r^2 &= - \lambda_r - \frac{r}{2} \nu_r (\lambda_r + \nu_r ) \\
  - \lambda_r - \frac{r}{2} \lambda_r \nu_r + \frac{r}{2}\nu_r^2 &= - \lambda_r - \frac{r}{2} \nu_r \lambda_r - \frac{r}{2} \nu_r^2 \\
  \frac{r}{2}\nu_r^2 &= - \frac{r}{2} \nu_r^2 \\
  r\nu_r^2 &= 0
\end{align*}
\begin{align}
  \nu_r &= 0
\end{align}

Applying this to Equation 14 we get the following differential equation:

\begin{align}
  - \lambda_r &= \frac{e^{\lambda} - 2}{r}
\end{align}

\section*{Final Equations}

\begin{align}
  - \lambda_r &= \frac{e^{\lambda} - 2}{r} \\
  \nu_r &= 0 \\
  \lambda_\tau &= 0
\end{align}


\end{document}